## E1
### 1.1 Weak Formulation

**Derivation:**
To obtain the weak formulation, we multiply the differential equation by a test function $v(x) \in V$ (where $v(0)=v(1)=0$) and integrate over the domain $(0,1)$:

$$\int_0^1 (-u'' - xu' + u)v \, dx = \int_0^1 fv \, dx$$

We integrate the first term by parts:
$$\int_0^1 -u''v \, dx = [-u'v]_0^1 + \int_0^1 u'v' \, dx$$
Since $v(0)=v(1)=0$, the boundary term $[-u'v]_0^1$ vanishes.

Substituting this back into the integral equation:
$$\int_0^1 u'v' \, dx - \int_0^1 xu'v \, dx + \int_0^1 uv \, dx = \int_0^1 fv \, dx$$

**Answer:**
The weak formulation is: find $u \in V$ such that $a(u,v) = F(v)$ for all $v \in V$.

**Definitions:**
* **Space $V$:** $H^1_0(0,1) = \{v \in H^1(0,1) : v(0) = v(1) = 0\}$
* **Bilinear form $a(u,v)$:**
  $$a(u,v) = \int_0^1 (u'v' - x u' v + uv) \, dx$$
* **Linear functional $F(v)$:**
  $$F(v) = \int_0^1 f v \, dx$$
  *(Note: Since $f(x)=0$ in the initial problem statement, $F(v)=0$. However, strictly speaking, the definition of the functional retains the general $f$.)*

---

### 1.2 Continuity and Coercivity

We use the standard norm on $V$: $\|v\|_V = \|v\|_{H^1} = \left(\|v'\|_{L^2}^2 + \|v\|_{L^2}^2\right)^{1/2}$.

**1. Continuity (Boundedness):**
We want to show $|a(u,v)| \leq M \|u\|_V \|v\|_V$.
Using the Cauchy-Schwarz inequality ($\int fg \leq \|f\|_0 \|g\|_0$) and noting that $|x| \leq 1$ on $(0,1)$:

$$
\begin{aligned}
|a(u,v)| &= \left| \int_0^1 u'v' - \int_0^1 xu'v + \int_0^1 uv \right| \\
&\leq \|u'\|_0 \|v'\|_0 + \sup|x| \cdot \|u'\|_0 \|v\|_0 + \|u\|_0 \|v\|_0 \\
&\leq \|u'\|_0 \|v'\|_0 + 1 \cdot \|u'\|_0 \|v\|_0 + \|u\|_0 \|v\|_0
\end{aligned}
$$

Since $\|u'\|_0 \leq \|u\|_V$ and $\|u\|_0 \leq \|u\|_V$ (and same for $v$):
$$|a(u,v)| \leq \|u\|_V \|v\|_V + \|u\|_V \|v\|_V + \|u\|_V \|v\|_V = 3 \|u\|_V \|v\|_V$$
**Continuity Constant:** $M = 3$ (Other constants are possible depending on the strictness of the inequality used).

**2. Coercivity (Ellipticity):**
We want to show $a(v,v) \geq \alpha \|v\|_V^2$.
$$a(v,v) = \int_0^1 (v')^2 \, dx - \int_0^1 x v' v \, dx + \int_0^1 v^2 \, dx$$

Let's analyze the middle term $-\int_0^1 x v' v \, dx$. Note that $v'v = \frac{1}{2}(v^2)'$. Integrating by parts:
$$-\int_0^1 x v' v \, dx = -\int_0^1 x \frac{1}{2} (v^2)' \, dx = - \left( \left[ \frac{1}{2} x v^2 \right]_0^1 - \int_0^1 \frac{1}{2} (x)' v^2 \, dx \right)$$
Because $v(1)=0$, the boundary term is 0.
$$= \frac{1}{2} \int_0^1 v^2 \, dx = \frac{1}{2} \|v\|_{L^2}^2$$

Substituting this back into $a(v,v)$:
$$a(v,v) = \|v'\|_{L^2}^2 + \frac{1}{2} \|v\|_{L^2}^2 + \|v\|_{L^2}^2 = \|v'\|_{L^2}^2 + \frac{3}{2} \|v\|_{L^2}^2$$
Since $\|v\|_V^2 = \|v'\|_{L^2}^2 + \|v\|_{L^2}^2$, we clearly have:
$$a(v,v) \geq 1 \cdot (\|v'\|_{L^2}^2 + \|v\|_{L^2}^2) = \|v\|_V^2$$
**Coercivity Constant:** $\alpha = 1$.

---

### 1.3 Exact Solution

The problem is:
$$-u'' - xu' + u = 0, \quad u(0)=u(1)=0$$

Based on the coercivity proved in 1.2 ($a(u,u) \geq \alpha \|u\|^2$), if $f=0$ (homogeneous equation), then $a(u,u) = F(u) = 0$.
Since $\alpha \|u\|_V^2 \leq a(u,u) = 0$, it implies $\|u\|_V = 0$.

Therefore, the exact solution is the trivial solution:
$$u(x) = 0$$

---

### 1.4 Finite Element Approximation

We approximate the problem using piecewise quadratic finite elements ($P_2$).
Let $h$ be the mesh size. According to standard Finite Element theory (CÃ©a's Lemma and Aubin-Nitsche lemma), for polynomials of degree $k=2$:

1.  **$H^1$ norm error:** The convergence order is $k = 2$ for the derivative.
    $$\|u - u_h\|_{H^1(0,1)} \leq C h^2 |u|_{H^3(0,1)}$$
    *(Note: Sometimes formulated as order $k$ for the $H^1$ norm, i.e., $O(h^2)$)*.

2.  **$L^2$ norm error:** The convergence order is $k+1 = 3$.
    $$\|u - u_h\|_{L^2(0,1)} \leq C h^3 |u|_{H^3(0,1)}$$

*(Note: Since the exact solution is $u=0$ and $f=0$, the numerical solution $u_h$ will also be exactly 0, making the error 0. However, the formulas above represent the theoretical error estimates for this finite element space).*

---

### 1.5 Derivation of f

We are given the exact solution $u_{ex} = x(1-x) = x - x^2$ and need to find $f$ for the equation:
$$-u'' - xu' + u = f$$

**Step 1: Calculate derivatives of $u_{ex}$**
$$u = x - x^2$$
$$u' = 1 - 2x$$
$$u'' = -2$$

**Step 2: Substitute into the LHS of the ODE**
$$-(-2) - x(1-2x) + (x-x^2)$$
$$= 2 - (x - 2x^2) + x - x^2$$
$$= 2 - x + 2x^2 + x - x^2$$

**Step 3: Simplify**
Combine like terms:
$$= 2 + (2x^2 - x^2) + (-x + x)$$
$$= 2 + x^2$$

**Answer:**
$$f(x) = x^2 + 2$$